\documentclass[a4paper,12pt]{article}

\usepackage{../header}
\newcommand{\school}{ntu}
\newcommand{\subject}{math}
\renewcommand{\year}{102}
\newcommand{\titlename}{\MakeUppercase{\school} \subject \ \year}

\fancypagestyle{mainmatter}{\rhead{\titlename}}
\pagestyle{mainmatter}
\CenterWallPaper{.50}{img/logo_ntu_recolor.jpg}
\newcommand{\ver}{\textsc{Version} 1.0} % Version number.

\begin{document}

\title{\LARGE{\textbf{Solutions}} \\
	\Huge{\textbf{\titlename}} \\
	\normalsize{\ver}
}
\author{}
\date{}

\maketitle

% Start of solutions.

\begin{enumerate}
	\item \begin{answer}{$\dag$} \textbf{WRONG}. Counterexample: \begin{equation}
            \begin{aligned}
                A & = \{1, \ 2, \ 3\} \\
                R & = \{(1, \ 2), \ (2, \ 1), \ (1, \ 1), \ (2, \ 2) \}    
            \end{aligned}
        \end{equation} $R$ is symmetric and transitive, but $R$ is NOT reflexive.
    \end{answer}
    \item \begin{answer}{$\dag$} Suppose \begin{equation}
            \begin{aligned}
                \Rightarrow & \ \begin{cases}
                    b_n & = \ n\text{-th character is} \ 0 \\
                    c_n & = \ n\text{-th character is} \ 1, \ \text{and} \ (n - 1)\text{-th character is} \ 0 \lor 2 \\
                    d_n & = \ n\text{-th character is} \ 2, \ \text{and} \ (n - 1)\text{-th character is} \ 0 \lor 1 \\
                \end{cases} \\
                \Rightarrow & \ a_n = b_n + c_n + d_n \\
                & \left(\begin{cases}
                    b_n & = a_{n - 1} \\
                    c_n & = a_{n - 1} - c_{n - 1} \ (\because \ n\text{-th character can NOT be} \ 1) \\
                    d_n & = a_{n - 1} - d_{n - 1} \ (\because \ n\text{-th character can NOT be} \ 2)
                \end{cases}\right)
            \end{aligned}
        \end{equation} Then, we have \begin{equation}
            \begin{aligned}
                a_n & = b_n + c_n + d_n \\
                & = a_{n - 1} + (a_{n - 1} - c_{n - 1}) + (a_{n - 1} - d_{n - 1}) \\
                & = 3 \times a_{n - 1} - c_{n - 1} - d_{n - 1} \ (\because \ a_{n - 1} = b_{n - 1} + c_{n - 1} + d_{n - 1}) \\
                & = 2 \times a_{n - 1} + b_{n - 1} \\
                & = 2 \times a_{n - 1} + b_{n - 2}
            \end{aligned}
        \end{equation}
    \end{answer}
    \item \quad \begin{enumerate}[label=(\alph*)]
        \item \begin{answer}{$\dag$}\begin{equation}
                1
            \end{equation} 
        \end{answer} Since it needs to contain all edges and all vertices.
        \item \begin{answer}{$\dag$}\begin{equation}
                \binom{n}{2}
            \end{equation} 
        \end{answer} Since it needs to be \textbf{complete}.
    \end{enumerate}
    \item \begin{answer}{$\dag$} Suppose $G$ have $n$ vertices. If $G = (\V, \E)$ is connected, \begin{equation}
            1 \le \deg(v) \le (n - 1), \ \forall \ v \in \V
        \end{equation} Since $|\V| = n$, and the possiblities of degree are $(n - 1)$, \begin{equation}
            \exists \ u, \ v \in \V, \ \text{s.t.} \ \deg(u) = \deg(v)
        \end{equation} Otherwise, if $G = (\V, \E)$ is NOT connected, suppose there exists $k$ vertices $u \in \V_1$ such that $\deg(u) = 0$, 
        so other $(n - k)$ vertices $v \in \V_2$ are connected, i.e., $\V = \V_1 + \V_2$. Then, we have \begin{equation}
            1 \le v \le (n - k - 1), \ \forall \ v \in \V_2
        \end{equation} Since $|\V_2| = n - k$, and the possiblities of degree are $(n - k - 1)$, \begin{equation}
            \exists \ v, \ w \in \V_2, \ \text{s.t.} \ \deg(v) = \deg(w)
        \end{equation} To summary, there are $2$ vertices in $G$ having equal degree.
    \end{answer}
    \item \begin{answer}{$\dag$} We have \begin{equation}
            \begin{aligned}
                & H \cap K \subseteq H, \ H \cap K \subseteq K \ (|H| = h, \ |K| = k, \ |H \cap K| = m) \\
                \Rightarrow & \ m | h, \ m | k \ (\text{by Lagrange Theorem}) \\
                \Rightarrow & \ m | \gcd(h, \ k) = 1 \\
                \Rightarrow & \ m = 1 \\
            \end{aligned}
        \end{equation} 
    \end{answer}
    \item We have \begin{equation}
        \begin{aligned}
            & \lambda_1\lambda_2 + \lambda_1\lambda_3 + \lambda_1\lambda_4 + \lambda_2\lambda_3 + \lambda_2\lambda_4 + \lambda_3\lambda_4 = \tr_2(\mat{A}) \\
            & = \begin{vmatrix}
                1 & 2 \\
                8 & 7
            \end{vmatrix} + \begin{vmatrix}
                1 & 3 \\
                1 & 5
            \end{vmatrix} + \begin{vmatrix}
                1 & 4 \\
                2 & 7
            \end{vmatrix} + \begin{vmatrix}
                7 & 6 \\
                4 & 5
            \end{vmatrix} + \begin{vmatrix}
                7 & 5 \\
                3 & 7
            \end{vmatrix} + \begin{vmatrix}
                5 & 8 \\
                6 & 7
            \end{vmatrix}
        \end{aligned}
    \end{equation}
    \begin{answer}{$\dag$}\begin{equation}
            24
        \end{equation} 
    \end{answer}
    \item \begin{answer}{$\dag$} Eigenvalue matrix: \begin{equation}
            \begin{bmatrix}
                3 \times \mat{\Lambda} & \mat{0} \\
                \mat{0} & 2 \times \mat{\Lambda}
            \end{bmatrix}
        \end{equation} Eigenvector matrix: \begin{equation}
            \begin{bmatrix}
                \mat{S} & \mat{0} \\
                \mat{0} & \mat{S}
            \end{bmatrix}
        \end{equation} 
    \end{answer}
    \item We have \begin{equation}
        \begin{aligned}
            \Ker(\mat{T}) & = \{\mat{A} \in \R^{n \times n} | \frac{\mat{A} + \mat{A}^\intercal}{2} = \mat{0}\} \\
            & = \{\mat{A} \in \R^{n \times n} | \mat{A} = -\mat{A}^\intercal\}
        \end{aligned}
    \end{equation}
    \begin{enumerate}[label=(\alph*)]
        \item \begin{answer}{$\dag$}\begin{equation}
                \{\mat{A} \in \R^{n \times n} | \mat{A} = -\mat{A}^\intercal\}
            \end{equation} 
        \end{answer} 
        \item \begin{answer}{$\dag$}\begin{equation}
                (\nul(\T), \ \rnk(\T)) = (\frac{n(n - 1)}{2}, \ \frac{n(n + 1)}{2})
            \end{equation} 
        \end{answer} 
    \end{enumerate}
    \item We have 
        \begin{flalign}
            & = \begin{vmatrix}
                a_0 & a_0 & \cdots & a_0 \\
                p_1(x_1) & p_1(x_2) & \cdots & p_1(x_n) \\
                \vdots & \vdots & \ddots & \vdots \\
                p_{n - 1}(x_1) & p_{n - 1}(x_2) & \cdots & p_{n - 1}(x_n)
            \end{vmatrix}_{n \times n}& \nonumber \\
            & (\because \ c_{n1}^{-1}, \ c_{n2}^{-1}, \ \cdots, \ c_{n(n - 1)}^{-1})& \nonumber \\
            & = \begin{vmatrix}
                0 & 0 & \cdots & a_0 \\
                p_1(x_1) - p_1(x_n) & p_1(x_2) - p_1(x_n) & \cdots & p_1(x_n) \\
                \vdots & \vdots & \ddots & \vdots \\
                p_{n - 1}(x_1) - p_{n - 1}(x_n) & p_{n - 1}(x_2) - p_{n - 1}(x_n) & \cdots & p_{n - 1}(x_n)
            \end{vmatrix}_{n \times n}& \nonumber \\
            & = (-1)^{n + 1}a_0 \begin{vmatrix}
                a_1(x_1 - x_n) & a_1(x_2 - x_n) & \cdots & a_1(x_{n - 1} - x_n) \\
                \sum\limits_{i = 1}^{2}a_i(x_1 - x_n)^i & \sum\limits_{i = 1}^{2}a_i(x_2 - x_n)^i & \cdots & \sum\limits_{i = 1}^{2}a_i(x_{n - 1} - x_n)^i \\
                \vdots & \vdots & \ddots & \vdots \\
                \sum\limits_{i = 1}^{n - 1}a_i(x_1 - x_n)^i & \sum\limits_{i = 1}^{n - 1}a_i(x_2 - x_n)^i & \cdots & \sum\limits_{i = 1}^{n - 1}a_i(x_{n - 1} - x_n)^i
            \end{vmatrix}_{{(n - 1)} \times {(n - 1)}}& \nonumber
        \end{flalign}
        \begin{flalign}
            & (\because \ r_{12}^{-1}, \ r_{13}^{-1}, \ \cdots, \ r_{1(n - 1)}^{-1}, \ r_{23}^{-1}, \ r_{24}^{-1}, \ \cdots, \ r_{2(n - 1)}^{-1}, \ r_{34}^{-1}, \ \cdots, \ r_{(n - 2)(n - 1)}^{-1})& \nonumber \\
            & = (-1)^{n + 1}a_0 \begin{vmatrix}
                a_1(x_1 - x_n) & a_1(x_2 - x_n) & \cdots & a_1(x_{n - 1} - x_n) \\
                a_2(x_1 - x_n)^2 & a_2(x_2 - x_n)^2 & \cdots & a_2(x_{n - 1} - x_n)^2 \\
                \vdots & \vdots & \ddots & \vdots \\
                a_{n - 1}(x_1 - x_n)^{n - 1} & a_{n - 1}(x_2 - x_n)^{n - 1} & \cdots & a_{n - 1}(x_{n - 1} - x_n)^{n - 1}
            \end{vmatrix}_{{(n - 1)} \times {(n - 1)}}& \nonumber \\
            & (\because \ r_{1}^{\frac{1}{a_1}}, \ r_{2}^{\frac{1}{a_2}}, \ \cdots, \ r_{n - 1}^{\frac{1}{a_{n - 1}}})& \nonumber \\
            & = (-1)^{n + 1}\displaystyle\prod_{i = 0}^{n - 1}a_i\begin{vmatrix}
                (x_1 - x_n) & (x_2 - x_n) & \cdots & (x_{n - 1} - x_n) \\
                (x_1 - x_n)^2 & (x_2 - x_n)^2 & \cdots & (x_{n - 1} - x_n)^2 \\
                \vdots & \vdots & \ddots & \vdots \\
                (x_1 - x_n)^{n - 1} & (x_2 - x_n)^{n - 1} & \cdots & (x_{n - 1} - x_n)^{n - 1}
            \end{vmatrix}_{{(n - 1)} \times {(n - 1)}}& \\
            & (\because \ c_1^{\frac{1}{x_1 - x_n}}, \ c_2^{\frac{1}{x_2 - x_n}}, \ \cdots, \ c_{n - 1}^{\frac{1}{x_{n - 1} - x_n}})& \nonumber \\
            & = (-1)^{n + 1}(\displaystyle\prod_{i = 0}^{n - 1}a_i)(\displaystyle\prod_{j = 1}^{n - 1}(x_j - x_n))\begin{vmatrix}
                1 & 1 & \cdots & 1 \\
                (x_1 - x_n) & (x_2 - x_n) & \cdots & (x_{n - 1} - x_n) \\
                \vdots & \vdots & \ddots & \vdots \\
                (x_1 - x_n)^{n - 2} & (x_2 - x_n)^{n - 2} & \cdots & (x_{n - 1} - x_n)^{n - 2}
            \end{vmatrix}_{{(n - 1)} \times {(n - 1)}}& \nonumber \\
            & (\because \ \text{Vandermonde matrix})& \nonumber \\
            & = (-1)^{n + 1}(\displaystyle\prod_{i = 0}^{n - 1}a_i)[(-1)^{n - 1}\displaystyle\prod_{j = 1}^{n - 1}(x_n - x_j)](\displaystyle\prod_{1 \le i \le j \le (n - 1)}(x_j - x_i))& \nonumber \\
            & = (\displaystyle\prod_{i = 0}^{n - 1}a_i)(\displaystyle\prod_{1 \le i \le j \le n}(x_j - x_i))& \nonumber
        \end{flalign}
    % \item We have \begin{equation}
    %     \begin{aligned}
    %         \det(\mat{A}) & = \begin{vmatrix}
    %             a_0 & a_0 & \cdots & a_0 \\
    %             p_1(x_1) & p_1(x_2) & \cdots & p_1(x_n) \\
    %             \vdots & \vdots & \ddots & \vdots \\
    %             p_{n - 1}(x_1) & p_{n - 1}(x_2) & \cdots & p_{n - 1}(x_n)
    %         \end{vmatrix} \ (\because \ c_{n1}^{-1}, \ c_{n2}^{-1}, \ \cdots, \ c_{n(n - 1)}^{-1})\\
    %         & = \begin{vmatrix}
    %             0 & 0 & \cdots & a_0 \\
    %             p_1(x_1) - p_1(x_n) & p_1(x_2) - p_1(x_n) & \cdots & p_1(x_n) \\
    %             \vdots & \vdots & \ddots & \vdots \\
    %             p_{n - 1}(x_1) - p_{n - 1}(x_n) & p_{n - 1}(x_2) - p_{n - 1}(x_n) & \cdots & p_{n - 1}(x_n)
    %         \end{vmatrix} \\
    %         & = (-1)^{n + 1}a_0 \begin{vmatrix}
    %             a_1(x_1 - x_n) & a_1(x_2 - x_n) & \cdots & a_1(x_{n - 1} - x_n) \\
    %             \sum\limits_{i = 1}^{2}a_i(x_1 - x_n)^i & \sum\limits_{i = 1}^{2}a_i(x_2 - x_n)^i & \cdots & \sum\limits_{i = 1}^{2}a_i(x_{n - 1} - x_n)^i \\
    %             \vdots & \vdots & \ddots & \vdots \\
    %             \sum\limits_{i = 1}^{n - 1}a_i(x_1 - x_n)^i & \sum\limits_{i = 1}^{n - 1}a_i(x_2 - x_n)^i & \cdots & \sum\limits_{i = 1}^{n - 1}a_i(x_{n - 1} - x_n)^i
    %         \end{vmatrix} \\
    %         & (\because \ r_{12}^{-1}, \ r_{13}^{-1}, \ \cdots, \ r_{1(n - 1)}^{-1}, \ r_{23}^{-1}, \ r_{24}^{-1}, \ \cdots, \ r_{2(n - 1)}^{-1}, \ r_{34}^{-1}, \ \cdots, \ r_{(n - 2)(n - 1)}^{-1}) \\
    %         & = (-1)^{n + 1}a_0 \begin{vmatrix}
    %             a_1(x_1 - x_n) & a_1(x_2 - x_n) & \cdots & a_1(x_{n - 1} - x_n) \\
    %             a_2(x_1 - x_n)^2 & a_2(x_2 - x_n)^2 & \cdots & a_2(x_{n - 1} - x_n)^2 \\
    %             \vdots & \vdots & \ddots & \vdots \\
    %             a_{n - 1}(x_1 - x_n)^{n - 1} & a_{n - 1}(x_2 - x_n)^{n - 1} & \cdots & a_{n - 1}(x_{n - 1} - x_n)^{n - 1}
    %         \end{vmatrix} \\
    %         & = (-1)^{n + 1}\displaystyle\prod_{i = 0}^{n - 1}a_i\begin{vmatrix}
    %             (x_1 - x_n) & (x_2 - x_n) & \cdots & (x_{n - 1} - x_n) \\
    %             (x_1 - x_n)^2 & (x_2 - x_n)^2 & \cdots & (x_{n - 1} - x_n)^2 \\
    %             \vdots & \vdots & \ddots & \vdots \\
    %             (x_1 - x_n)^{n - 1} & (x_2 - x_n)^{n - 1} & \cdots & (x_{n - 1} - x_n)^{n - 1}
    %         \end{vmatrix} \\
    %         & \overset{c_1^{\frac{1}{x_1 - x_n}}, \ c_2^{\frac{1}{x_2 - x_n}}, \ \cdots, \ c_{n - 1}^{\frac{1}{x_{n - 1} - x_n}}}= \\
    %         & (-1)^{n + 1}(\displaystyle\prod_{i = 0}^{n - 1}a_i)(\displaystyle\prod_{j = 1}^{n - 1}(x_j - x_n))\begin{vmatrix}
    %             1 & 1 & \cdots & 1 \\
    %             (x_1 - x_n) & (x_2 - x_n) & \cdots & (x_{n - 1} - x_n) \\
    %             \vdots & \vdots & \ddots & \vdots \\
    %             (x_1 - x_n)^{n - 2} & (x_2 - x_n)^{n - 2} & \cdots & (x_{n - 1} - x_n)^{n - 2}
    %         \end{vmatrix} \\
    %         & = (-1)^{n + 1}(\displaystyle\prod_{i = 0}^{n - 1}a_i)[(-1)^{n - 1}\displaystyle\prod_{j = 1}^{n - 1}(x_n - x_j)](\displaystyle\prod_{1 \le i \le j \le (n - 1)}(x_j - x_i)) \\
    %         & (\because \ \text{Vandermonde matrix}) \\
    %         & = (\displaystyle\prod_{i = 0}^{n - 1}a_i)(\displaystyle\prod_{1 \le i \le j \le n}(x_j - x_i))           
    %     \end{aligned}
    % \end{equation}
    \begin{answer}{$\dag$}\begin{equation}
            (\displaystyle\prod_{i = 0}^{n - 1}a_i)(\displaystyle\prod_{1 \le i \le j \le n}(x_j - x_i))
        \end{equation} 
    \end{answer}
    \item We have \begin{equation}
        \begin{aligned}
            \Rightarrow & \ \alpha^2 = \frac{1}{2} \times \alpha - \frac{1}{2} \\
            \Rightarrow & \ \alpha = -\frac{1}{2} \lor \alpha = 1 \\
            \Rightarrow & \ B_n = c \times (-\frac{1}{2})^n + d \times (1)^n
        \end{aligned}
    \end{equation} And, we have \begin{equation}
        \begin{aligned}
            & \begin{cases}
                B_0 = 0 = c + d \\
                B_1 = \frac{1}{2} = -\frac{1}{2} \times c + d
            \end{cases} \\
            \Rightarrow & \ c = -\frac{1}{3}, \ d = \frac{1}{3}
        \end{aligned}
    \end{equation}
    \begin{answer}{$\dag$}\begin{equation}
            B_k = \frac{1}{3} - \frac{1}{3} \times (-\frac{1}{2})^k, \ \lim_{k \rightarrow \infty} B_k = \frac{1}{3}
        \end{equation} 
    \end{answer}
    \item We have \begin{enumerate}[label=(\alph*)]
        \item True.
        \item False.
        \item False, since $\vec{0} \in \spc{W}_1 \rightarrow \vec{0} \neq (\V - \spc{W}_1)$.
        \item False, since $\vec{0} \in \spc{W}_1 \rightarrow \vec{0} \neq (\V - \spc{W}_1)$.
        \item False.
    \end{enumerate}
    \item We have \begin{enumerate}[label=(\alph*)]
        \item True.
        \item True.
        \item True.
        \item False.
        \item False.
    \end{enumerate}
\end{enumerate}

% End of solutions.

\end{document}

